HepLean/PerturbationTheory/FieldStruct/Contractions/Involutions.lean
@@ -1,0 +1,153 @@
+/-
+Copyright (c) 2025 Joseph Tooby-Smith. All rights reserved.
+Released under Apache 2.0 license as described in the file LICENSE.
+Authors: Joseph Tooby-Smith
+-/
+import HepLean.PerturbationTheory.FieldStruct.Contractions.Uncontracted
+import HepLean.PerturbationTheory.FieldStruct.TimeOrder
+import HepLean.PerturbationTheory.FieldStruct.TimeContraction
+import HepLean.PerturbationTheory.FieldStruct.Contractions
+/-!
+
+# Involution associated with a contraction
+
+
+-/
+
+namespace FieldStruct
+variable {𝓕 : FieldStruct}
+namespace ContractionsNat
+variable {n : ℕ} (c : ContractionsNat n)
+open HepLean.List
+open FieldStatistic
+
+def toInvolution : {f : Fin n → Fin n // Function.Involutive f} :=
+  ⟨fun i => if h : (c.getDual? i).isSome then (c.getDual? i).get h else i, by
+    intro i
+    by_cases h : (c.getDual? i).isSome
+    · simp [h]
+    · simp [h]⟩
+
+def fromInvolution (f : {f : Fin n → Fin n // Function.Involutive f}) : ContractionsNat n :=
+  ⟨Finset.univ.filter (fun a => a.card = 2 ∧ ∃ i, {i, f.1 i} = a), by
+  intro a
+  simp
+  intro h1 _ _
+  exact h1, by
+  intro a ha b hb
+  simp at ha hb
+  obtain ⟨i, hai⟩ := ha.2
+  subst hai
+  obtain ⟨j, hbj⟩ := hb.2
+  subst hbj
+  by_cases h : i = j
+  · subst h
+    simp
+  · by_cases hi : i = f.1 j
+    · subst hi
+      simp
+      rw [f.2]
+      rw [@Finset.pair_comm]
+    · apply Or.inr
+      simp
+      apply And.intro
+      · apply And.intro
+        · exact fun a => h a.symm
+        · by_contra hn
+          subst hn
+          rw [f.2 i] at hi
+          simp at hi
+      · apply And.intro
+        · exact fun a => hi a.symm
+        · rw [Function.Injective.eq_iff]
+          exact fun a => h (id (Eq.symm a))
+          exact Function.Involutive.injective f.2⟩
+
+@[simp]
+lemma fromInvolution_getDual?_isSome (f : {f : Fin n → Fin n // Function.Involutive f}) (i : Fin n) :
+  ((fromInvolution f).getDual? i).isSome ↔ f.1 i ≠ i := by
+  rw [getDual?_isSome_iff]
+  apply Iff.intro
+  · intro h
+    obtain ⟨a, ha⟩ := h
+    have ha2 := a.2
+    simp  [fromInvolution, -Finset.coe_mem] at ha2
+    obtain ⟨j, h⟩ := ha2.2
+    rw [← h] at ha
+    have hj : f.1 j ≠ j := by
+      by_contra hn
+      rw [hn] at h
+      rw [← h] at ha2
+      simp at ha2
+    simp at ha
+    rcases ha with ha | ha
+    · subst ha
+      exact hj
+    · subst ha
+      rw [f.2 ]
+      exact id (Ne.symm hj)
+  · intro hi
+    use ⟨{i, f.1 i}, by
+      simp [fromInvolution]
+      rw [Finset.card_pair (id (Ne.symm hi))]⟩
+    simp
+
+lemma fromInvolution_getDual?_eq_some (f : {f : Fin n → Fin n // Function.Involutive f}) (i : Fin n)
+    (h : ((fromInvolution f).getDual? i).isSome) :
+   ((fromInvolution f).getDual? i) = some (f.1 i)  := by
+  rw [@getDual?_eq_some_iff_mem]
+  simp [fromInvolution]
+  apply Finset.card_pair
+  simp at h
+  exact fun a => h (id (Eq.symm a))
+
+@[simp]
+lemma fromInvolution_getDual?_get (f : {f : Fin n → Fin n // Function.Involutive f}) (i : Fin n)
+    (h : ((fromInvolution f).getDual? i).isSome) :
+   ((fromInvolution f).getDual? i).get h =  (f.1 i)  := by
+  have h1 := fromInvolution_getDual?_eq_some f i h
+  exact Option.get_of_mem h h1
+
+lemma toInvolution_fromInvolution : fromInvolution c.toInvolution = c :=  by
+  apply Subtype.eq
+  simp [fromInvolution, toInvolution]
+  ext a
+  simp
+  apply Iff.intro
+  · intro h
+    obtain ⟨i, hi⟩ := h.2
+    split at hi
+    · subst hi
+      simp
+    · simp at hi
+      subst hi
+      simp at h
+  · intro ha
+    apply And.intro (c.2.1 a ha)
+    use c.fstFieldOfContract ⟨a, ha⟩
+    simp
+    change _ = (⟨a, ha⟩ : c.1).1
+    conv_rhs => rw [finset_eq_fstFieldOfContract_sndFieldOfContract]
+
+lemma fromInvolution_toInvolution  (f : {f : Fin n → Fin n // Function.Involutive f}) :
+    (fromInvolution f).toInvolution = f :=  by
+  apply Subtype.eq
+  funext i
+  simp only [toInvolution,  ne_eq, dite_not]
+  split
+  · rename_i h
+    simp
+  · rename_i h
+    simp at h
+    exact id (Eq.symm h)
+
+def equivInvolution : ContractionsNat n ≃ {f : Fin n → Fin n // Function.Involutive f} where
+  toFun := toInvolution
+  invFun := fromInvolution
+  left_inv := toInvolution_fromInvolution
+  right_inv := fromInvolution_toInvolution
+
+
+end ContractionsNat
+
+end FieldStruct
