HepLean/PerturbationTheory/FieldStruct/Contractions/IsFull.lean
@@ -1,0 +1,62 @@
+/-
+Copyright (c) 2025 Joseph Tooby-Smith. All rights reserved.
+Released under Apache 2.0 license as described in the file LICENSE.
+Authors: Joseph Tooby-Smith
+-/
+import HepLean.PerturbationTheory.FieldStruct.Contractions.Involutions
+import HepLean.PerturbationTheory.FieldStruct.TimeOrder
+import HepLean.PerturbationTheory.FieldStruct.TimeContraction
+import HepLean.PerturbationTheory.FieldStruct.Contractions
+import HepLean.Mathematics.Fin.Involutions
+/-!
+
+# Full involutions
+
+
+-/
+
+namespace FieldStruct
+variable {𝓕 : FieldStruct}
+namespace ContractionsNat
+variable {n : ℕ} (c : ContractionsNat n)
+open HepLean.List
+open FieldStatistic
+
+def IsFull : Prop := c.uncontracted = ∅
+
+instance : Decidable (IsFull c) :=  decEq c.uncontracted ∅
+
+lemma isFull_iff_equivInvolution_no_fixed_point :
+    IsFull c ↔ ∀ (i : Fin n), (equivInvolution c).1 i ≠ i := by
+  simp [IsFull]
+  rw [Finset.eq_empty_iff_forall_not_mem]
+  simp [equivInvolution, toInvolution, uncontracted]
+
+def isFullInvolutionEquiv : {c : ContractionsNat n // IsFull c} ≃
+    {f : Fin n → Fin n // Function.Involutive f ∧ (∀ i, f i ≠ i)} where
+  toFun c := ⟨equivInvolution c.1, by
+    apply And.intro (equivInvolution c.1).2
+    rw [← isFull_iff_equivInvolution_no_fixed_point]
+    exact c.2⟩
+  invFun f := ⟨equivInvolution.symm ⟨f.1, f.2.1⟩, by
+    rw [isFull_iff_equivInvolution_no_fixed_point]
+    simpa using f.2.2⟩
+  left_inv c := by simp
+  right_inv f := by simp
+
+open Nat
+
+theorem card_of_isfull_even (he : Even n) :
+    Fintype.card {c : ContractionsNat n // IsFull c} = (n - 1)‼ := by
+  rw [Fintype.card_congr (isFullInvolutionEquiv)]
+  exact HepLean.Fin.involutionNoFixed_card_even n he
+
+theorem card_of_isfull_odd (ho : Odd n) :
+    Fintype.card  {c : ContractionsNat n // IsFull c} = 0 := by
+  rw [Fintype.card_congr (isFullInvolutionEquiv)]
+  exact HepLean.Fin.involutionNoFixed_card_odd n ho
+
+
+end ContractionsNat
+
+end FieldStruct
